\section{Schmidt Number}
\label{schmidtAppendix}
\subsection{Definition}
Here we recall some quantum mechanics in order to derive a way to find the purity of experimental data. Starting with some arbitrary state $\psi$:
\begin{align}
|\psi \rangle &= \sum_{i,j}\alpha(i,j)|i\rangle_A\otimes|j\rangle_B 
\end{align}
The schimdt number $K$ of this state measures the degree of entanglement. If $K=1$ then you can find $|\psi \rangle  = |\xi \rangle\otimes |\eta \rangle$ and for $K>1$ you can find: 
\begin{align}
|\psi \rangle &=\sum_{i} r_i|\xi_i \rangle_A\otimes |\eta_i \rangle_B
\end{align}
An expression for $K$ can be found using the density matrix for $\psi$:
\begin{align}
\rho_{AB} &=|\psi \rangle \langle\psi| = \sum_{i,j,k,l}\alpha(i,j)\alpha^*(k,l)|i\rangle\langle k| \otimes|j\rangle \langle l| \\
\rho_{A} &=\Tr_B(\rho_{AB}) = \sum_{i,j,k}\alpha(i,j)\alpha^*(k,j)|i\rangle \langle k|  \\
\rho_{A}^2 &= \sum_{i',j',k'}\sum_{i,j,k}\alpha(i,j)\alpha(k,j)\alpha^*(i',j')\alpha^*(k',j')|i\rangle \langle k|i'\rangle \langle k'|  \\
&= \sum_{j',k'}\sum_{i,j,k}\alpha(i,j)\alpha^*(k,j)\alpha(k,j')\alpha^*(k',j')|i\rangle \langle k'|  \\
\Tr_A(\rho_{A}^2)&= \sum_{i,j,k,j'}\alpha(i,j)\alpha^*(k,j)\alpha(k,j')\alpha^*(i,j')  \\
\end{align}
For a unentangled $\psi$ we know that $\Tr_A(\rho_{A}^2)=1$ For $\psi$ entangled this will be smaller than 1 (proof comes from the property of the density operator that its eigenvalues are all smaller than 1). This fits the definition of the purity of a quantum state hence we can write:
\begin{align} \label{theShit}
P = \frac{1}{K}&= \sum_{i,j,k,l}\alpha(i,j)\alpha^*(k,j)\alpha(k,l)\alpha^*(i,l)
\end{align}
\subsection{Calculation from experimental data}
\subsubsection{Trace method}
In the lab we can measure $|\phi(\omega_1,\omega_2)|^2$, here we outline how to extract the schimdt number from this set of values. Taking the positive square root of the matrix of values obtained from the lab you have a matrix ${\bf f}$ given by:
\begin{align}
{\bf f}&=\sum_{\omega_1,\omega_2}\phi(\omega_1,\omega_2)|\omega_1\rangle\langle\omega_2|
\end{align}
This is an unorthodox method of writing the wavefunction but it turns out to be useful and so we now calculate some combinations of the matrix in order to mimic the work above.
\begin{align}\label{rhoA}
{\bf f}^{\dagger}{\bf f}&=\sum_{\omega_1,\omega_2,\omega_3}\phi(\omega_1,\omega_2)\phi(\omega_3,\omega_2)|\omega_1\rangle\langle\omega_3|
\end{align}
\begin{align}
({\bf f}^{\dagger}{\bf f})^2&=\sum_{\omega_1,\omega_2,\omega_3,\omega_4,\omega_5,\omega_6}\phi(\omega_1,\omega_2)\phi(\omega_3,\omega_2)\phi(\omega_4,\omega_5)\phi(\omega_6,\omega_5)|\omega_1\rangle\langle\omega_3|\omega_4\rangle\langle\omega_6|\\
({\bf f}^{\dagger}{\bf f})^2&=\sum_{\omega_1,\omega_2,\omega_3,\omega_4,\omega_5,\omega_6}\phi(\omega_1,\omega_2)\phi(\omega_3,\omega_2)\phi(\omega_3,\omega_5)\phi(\omega_6,\omega_5)|\omega_1\rangle\langle\omega_6|\\
\Tr\left [({\bf f}^{\dagger}{\bf f})^2 \right ]&=\sum_{\omega_1,\omega_2,\omega_3,\omega_4}\phi(\omega_1,\omega_2)\phi(\omega_3,\omega_2)\phi(\omega_3,\omega_4)\phi(\omega_1,\omega_4)
\end{align}
It is now visible that equation \ref{theShit} is of exactly the same form as $\Tr\left [({\bf f}^{\dagger}{\bf f})^2 \right ]$ (barring the conjugates but this is okay since $\phi$ is real.) Taking the parallel further it can be seen that equation \ref{rhoA} is of the form of a reduced density matrix. Here we must make sure to normalise to make sure this is a valid reduced density matrix. The normalisation is:
\begin{align}
N = \Tr\left [{\bf f}^{\dagger}{\bf f} \right ]&=\sum_{\omega_1,\omega_2}\phi(\omega_1,\omega_2)^2
\end{align}
Giving:
\begin{align}
\rho_A = \frac{{\bf f}^{\dagger}{\bf f}}{N}
\end{align}
We can then write:
\begin{align}
\frac{1}{K}=\frac{\Tr\left [({\bf f}^{\dagger}{\bf f})^2 \right ]}{\Tr\left [{\bf f}^{\dagger}{\bf f} \right ]^2}
\end{align}
\subsubsection{Alternate implementation with SVD decomposition} \label{svdAppendix}
Taking the SVD decomposition of ${\bf f}$ gives:
\begin{align}
{\bf f}&=\sum_{i}|u_i\rangle s_i\langle v_i|
\end{align}
Where $\lambda_i$ are the singular values. From wikipedia it turns out that $s_i^2$ are the eigenvalues of  ${\bf f}^{\dagger}{\bf f}$ which is also equal to the reduced density operator. Following the steps of the previous section then gives:
\begin{align}
{\bf f}^{\dagger}{\bf f}&=\sum_{i}|i\rangle \lambda^2_i\langle i|\\
({\bf f}^{\dagger}{\bf f})^2&=\sum_{i}|i\rangle \lambda^4_i\langle i|
\end{align}
And so:
\begin{align}
\frac{1}{K}=\frac{\Tr\left [({\bf f}^{\dagger}{\bf f})^2 \right ]}{\Tr\left [{\bf f}^{\dagger}{\bf f} \right ]^2}=\frac{\sum_{i}\lambda^4_i}{\left ( \sum_{j}\lambda^2_j \right )^2}=\sum_{i}\left (\frac{\lambda^2_i}{ \sum_{j}\lambda_j^2 }\right )^2
\end{align}